Memory (including sizeof, offsets and type size constants) all done.

holsrcs/memoryScript.sml
@@ -9,8 +9,8 @@ open HolKernel boolLib Parse bossLib BasicProvers
 open boolSimps
 
 (* Standard HOL ancestory theories *)
-open arithmeticTheory pred_setTheory
-local open wordsTheory in end
+open arithmeticTheory pred_setTheory integerTheory
+local open wordsTheory integer_wordTheory finite_mapTheory in end
 
 (* C++ ancestor theories  *)
 open typesTheory
@@ -72,47 +72,22 @@ val _ = type_abbrev("byte", ``:bool ** byte_index``)
     sizes of integral and pointer types
    ---------------------------------------------------------------------- *)
 
-val two_lemma = prove(
-  --`!n. 2 <= n ==> ?m. n = SUC (SUC m)`--,
-  REPEAT STRIP_TAC THEN Q.EXISTS_TAC `n - 2` THEN
-  ASM_SIMP_TAC (srw_ss() ++ ARITH_ss) []);
-val exp_mono_lemma = prove(
-  --`!b n. 2 <= b ==> b EXP n < b EXP (n + 1)`--,
-  REPEAT STRIP_TAC THEN IMP_RES_TAC two_lemma THEN SRW_TAC [][] THEN
-  ASSUME_TAC (SPECL [--`n:num`--, --`m:num`--] LESS_EXP_SUC_MONO) THEN
-  FULL_SIMP_TAC (srw_ss()) [ADD1]);
-val exp_mono_lemma2 = prove(
-  --`!b d x. 2 <= b /\ 0 < d ==> b EXP x < b EXP (x + d)`--,
-  Induct_on `d` THEN
-  REWRITE_TAC [prim_recTheory.LESS_REFL] THEN
-  REPEAT STRIP_TAC THEN
-  REPEAT_TCL STRIP_THM_THEN SUBST_ALL_TAC
-    (SPEC (--`d:num`--) num_CASES) THEN
-  FULL_SIMP_TAC (srw_ss() ++ ARITH_ss) [exp_mono_lemma, ADD1] THEN
-  REWRITE_TAC [DECIDE (--`n + (x + 2n) = (n + (x + 1)) + 1`--)] THEN
-  PROVE_TAC [LESS_TRANS, exp_mono_lemma]);
-val exp_monotonicity = prove(
-  --`!b x y. 2 <= b /\ x < y ==> b EXP x < b EXP y`--,
-  REPEAT STRIP_TAC THEN IMP_RES_TAC LESS_ADD_1 THEN
-  ASM_REWRITE_TAC [] THEN MATCH_MP_TAC exp_mono_lemma2 THEN
-  ASM_SIMP_TAC (srw_ss() ++ ARITH_ss) []);
+open logrootTheory
 val log_lemma = prove(
-  --`!b x. 2 <= b ==> ?n. x <= b EXP n`--,
-  Induct_on `x` THEN REPEAT STRIP_TAC THENL [
-    Q.EXISTS_TAC `0` THEN SIMP_TAC (srw_ss()) [],
-    RES_TAC THEN
-    IMP_RES_THEN (ASSUME_TAC o SPEC_ALL) exp_mono_lemma THEN
-    Q.EXISTS_TAC `SUC n` THEN FULL_SIMP_TAC (srw_ss() ++ ARITH_ss) [ADD1]
-  ]);
+  ``!b x. 2 <= b ==> ?n. x <= b EXP n``,
+  REPEAT STRIP_TAC THEN
+  Q.EXISTS_TAC `SUC(LOG b x)` THEN
+  Cases_on `x = 0` THEN1 SRW_TAC [][] THEN
+  ASSUME_TAC (Q.SPECL [`b`, `x`] LOG) THEN
+  DECIDE_TAC)
 val x_less_CHAR_BIT = prove(
   --`!x. x < 8 ==> x < CHAR_BIT`--,
   ASSUME_TAC CHAR_BIT THEN DECIDE_TAC);
 val exp2CB_gt_2 = prove(
   --`2 <= 2 EXP CHAR_BIT`--,
-  Q_TAC SUFF_TAC `2 < 2 EXP CHAR_BIT` THEN1 DECIDE_TAC THEN
-  MATCH_MP_TAC LESS_EQ_LESS_TRANS THEN Q.EXISTS_TAC `2 ** 1` THEN
-  CONJ_TAC THEN1 SRW_TAC [][] THEN
-  MATCH_MP_TAC exp_monotonicity THEN SIMP_TAC (srw_ss()) [x_less_CHAR_BIT]);
+  Q_TAC SUFF_TAC `1 <= CHAR_BIT` THEN1
+    METIS_TAC [EXP_BASE_LE_MONO, DECIDE ``1n < 2``, EXP_1] THEN
+  ASSUME_TAC x_less_CHAR_BIT THEN intLib.ARITH_TAC)
 
 fun size_spec n t = let
   val sz_t = rand (rator (#2 (dest_exists t)))
@@ -120,49 +95,77 @@ in
   Rsyntax.new_specification {
     consts = [{const_name = n, fixity = Prefix}],
     name = n,
-    sat_thm = prove(t, SIMP_TAC list_ss [integerTheory.INT_EXP] THEN
+    sat_thm = prove(t, SIMP_TAC list_ss [INT_EXP] THEN
                        Q.SUBGOAL_THEN `?n. ^sz_t = &n`
                         (CHOOSE_THEN SUBST_ALL_TAC) THENL [
-                          PROVE_TAC [integerTheory.NUM_POSINT_EXISTS,
-                                     integerTheory.INT_LE_TRANS,
-                                     type_size_constants,
-                                     integerTheory.INT_LE,
+                          PROVE_TAC [NUM_POSINT_EXISTS, INT_LE_TRANS,
+                                     type_size_constants, INT_LE,
                                      ZERO_LESS_EQ],
-                          SIMP_TAC list_ss [integerTheory.INT_LE,
-                                           log_lemma, exp2CB_gt_2]
+                          SIMP_TAC list_ss [INT_LE, log_lemma, exp2CB_gt_2]
                        ])}
 end;
 val short_size = size_spec "short_size"
   (--`?x. USHRT_MAX <= (2 ** CHAR_BIT) ** x`--);
+val short_size_nonzero = store_thm(
+  "short_size_nonzero",
+  ``0 < short_size``,
+  Q_TAC SUFF_TAC `~(short_size = 0)` THEN1 DECIDE_TAC THEN
+  ASSUME_TAC short_size THEN STRIP_TAC THEN
+  FULL_SIMP_TAC (srw_ss()) [EXP] THEN
+  `65535 <= USHRT_MAX` by SRW_TAC [][type_size_constants] THEN
+  intLib.ARITH_TAC)
+
 val int_size = size_spec "int_size"
   (--`?x. UINT_MAX <= (2 ** CHAR_BIT) ** x`--);
+val int_size_nonzero = store_thm(
+  "int_size_nonzero",
+  ``0 < int_size``,
+  Q_TAC SUFF_TAC `~(int_size = 0)` THEN1 DECIDE_TAC THEN
+  ASSUME_TAC int_size THEN STRIP_TAC THEN
+  FULL_SIMP_TAC (srw_ss()) [EXP] THEN
+  `65535 <= UINT_MAX` by SRW_TAC [][type_size_constants] THEN
+  intLib.ARITH_TAC)
+
 val long_size = size_spec "long_size"
-  (--`?x. ULONG_MAX <= (2 ** CHAR_BIT) ** x`--);
+  (--`?x. ULONG_MAX <= (2 ** CHAR_BIT) ** x`--)
+val long_size_nonzero = store_thm(
+  "long_size_nonzero",
+  ``0 < long_size``,
+  Q_TAC SUFF_TAC `~(long_size = 0)` THEN1 DECIDE_TAC THEN
+  ASSUME_TAC long_size THEN STRIP_TAC THEN
+  FULL_SIMP_TAC (srw_ss()) [EXP] THEN
+  `4294967295 <= ULONG_MAX` by SRW_TAC [][type_size_constants] THEN
+  intLib.ARITH_TAC)
 
 (* bit = "basic integral type" here *)
 val bit_size = Define`
   (bit_size Char = 1) /\ (bit_size Short = short_size) /\
   (bit_size Int = int_size) /\ (bit_size Long = long_size)
 `;
-val ptr_size = Rsyntax.new_specification {
-  consts = [{const_name = "voidptr_size", fixity = Prefix},
-            {const_name = "ptr_size", fixity = Prefix}],
-  name = "ptr_size",
-  sat_thm = CONV_RULE (QUANT_CONV SKOLEM_CONV) (prove(
-    --`?v. !t. ?x.
-          ((t = Unsigned Char) \/ (t = Signed Char) \/
-           (t = Void) ==> (x = v)) /\ 1n <= x /\ x <= v`--,
-    Q.EXISTS_TAC `1` THEN GEN_TAC THEN Q.EXISTS_TAC `1` THEN
-    SIMP_TAC list_ss []))};
-(* val ptr_size = Rsyntax.new_specification {
-  consts = [{const_name = "ptr_size", fixity = Prefix}],
-  name = "ptr_size",
-  sat_thm = prove(--`?x. 1n <= x`--, SIMP_TAC hol_ss [LESS_OR_EQ])}; *)
 
-val int_size_def = Define`
-  (int_size (Signed x) = bit_size x) /\
-  (int_size (Unsigned x) = bit_size x) /\
-  (int_size BChar = 1)
+val bool_size = new_specification(
+  "bool_size",
+  ["bool_size"],
+  prove(``?n. 1n <= n``, intLib.ARITH_TAC))
+
+
+(* pointer to void can contain all other pointers to objects (3.9.2 s4)
+   "void *" has same rep and alignment as "char *" (3.9.2 s4)
+*)
+val ptr_size = new_specification (
+  "ptr_size",
+  ["ptr_size"],
+  prove(``?f. (f BChar = f Void) /\
+              !ty. (object_type ty ==> f ty <= f Void) /\
+                   1n <= f ty``,
+        Q.EXISTS_TAC `K 1` THEN SRW_TAC [][]))
+
+(* size of integral types *)
+val int_sizeof_def = Define`
+  (int_sizeof (Signed x) = bit_size x) /\
+  (int_sizeof (Unsigned x) = bit_size x) /\
+  (int_sizeof BChar = 1) /\
+  (int_sizeof Bool = bool_size)
 `;
 
 (* There are a few encoding functions required to turn bytes from
@@ -233,527 +236,323 @@ val int_size_def = Define`
 (* show that rep_int and int_value functions of the desired behaviours
    exist *)
 
+(* currently this is NOT COMPLETE - not all properties are listed *)
+val char_onecomp_def = Define`
+  char_onecomp = (SCHAR_MIN = ~SCHAR_MAX)
+`;
+open wordsTheory
+val mod_add_lemma = prove(
+  ``0 < c ==> (x MOD c = (x + c) MOD c)``,
+  METIS_TAC [ADD_MODULUS_LEFT])
+val SUB_RIGHT_ADD' = prove(
+  ``x - y + (z : num) = if y <= x then x + z - y else z``,
+  DECIDE_TAC);
+
+val mod_sub_lemma = prove(
+  ``0 < c /\ y <= x ==> ((x - y) MOD c = (x MOD c + (c - y MOD c)) MOD c)``,
+  STRIP_TAC THEN
+  Q.SPEC_THEN `c` MP_TAC arithmeticTheory.DIVISION THEN ASM_REWRITE_TAC [] THEN
+  DISCH_THEN (fn th =>
+                 (MAP_EVERY (fn q => Q.SPEC_THEN q STRIP_ASSUME_TAC th)
+                            [`x`,`y`])) THEN
+  Q.ABBREV_TAC `q = y DIV c` THEN POP_ASSUM (K ALL_TAC) THEN
+  Q.ABBREV_TAC `r = y MOD c` THEN POP_ASSUM (K ALL_TAC) THEN
+  Q.ABBREV_TAC `s = x DIV c` THEN POP_ASSUM (K ALL_TAC) THEN
+  Q.ABBREV_TAC `t = x MOD c` THEN POP_ASSUM (K ALL_TAC) THEN
+  ASM_REWRITE_TAC [arithmeticTheory.SUB_PLUS] THEN
+  `q * c <= s * c`
+      by (SRW_TAC [ARITH_ss][LE_MULT_RCANCEL] THEN
+          SPOSE_NOT_THEN ASSUME_TAC THEN
+          `s + 1 <= q` by DECIDE_TAC THEN
+          `(s + 1) * c <= q * c`
+             by SRW_TAC [ARITH_ss][LE_MULT_RCANCEL] THEN
+          `s * c + t < q * c`
+             by (FULL_SIMP_TAC bool_ss [RIGHT_ADD_DISTRIB, MULT_CLAUSES] THEN
+                 DECIDE_TAC) THEN
+          DECIDE_TAC) THEN
+  `r <= (s - q) * c + t` by DECIDE_TAC THEN
+  `s * c + t - q * c = (s - q) * c + t`
+     by ASM_SIMP_TAC bool_ss [RIGHT_SUB_DISTRIB, SUB_RIGHT_ADD'] THEN
+  `((s-q)*c + t - r) MOD c = ((s-q)*c + t - r + c) MOD c`
+      by PROVE_TAC [mod_add_lemma] THEN
+  `(s - q) * c + t - r + c = (s - q) * c + (t + (c - r))`
+      by ASM_SIMP_TAC bool_ss
+                      [SUB_RIGHT_ADD',
+                       DECIDE ``r < (z:num) ==>
+                                (x + y + z - r = x + (y + (z - r)))``] THEN
+  ASM_SIMP_TAC bool_ss [MOD_TIMES]);
+
+val word_sub_n2w_1 = prove(
+  ``m <= n ==> (n2w n - n2w m = n2w (n - m))``,
+  SRW_TAC [][word_sub_def, word_2comp_def, word_add_n2w] THEN
+  `0 < 2 ** dimindex (UNIV : 'a set)` by SRW_TAC [][] THEN
+  SRW_TAC [][mod_sub_lemma] THEN
+  Q_TAC SUFF_TAC `!x y c. 0 < c ==> ((x MOD c + y) MOD c = (x + y) MOD c)`
+        THEN1 SRW_TAC [][] THEN
+  METIS_TAC [MOD_MOD, MOD_PLUS])
+
+val CHAR_BIT_BOUNDS = store_thm(
+  "CHAR_BIT_BOUNDS",
+  ``1n <= 2 ** CHAR_BIT /\ 2n <= 2 ** CHAR_BIT /\ 1 <= CHAR_BIT``,
+  `1 <= CHAR_BIT` by (ASSUME_TAC CHAR_BIT THEN DECIDE_TAC) THEN
+  SRW_TAC [][DECIDE ``1n <= x = 0 < x``] THEN
+  METIS_TAC [EXP_1, EXP_BASE_LE_MONO, DECIDE ``1n < 2``]);
+
+val TWICE_SCHAR_MAX = store_thm(
+  "TWICE_SCHAR_MAX",
+  ``2n * 2 ** (CHAR_BIT - 1) = 2 ** CHAR_BIT``,
+  `CHAR_BIT = SUC (CHAR_BIT - 1)`
+     by (ASSUME_TAC CHAR_BIT_BOUNDS THEN DECIDE_TAC) THEN
+  METIS_TAC [EXP, MULT_COMM])
+
+val SCHAR_MAX = store_thm(
+  "SCHAR_MAX",
+  ``SCHAR_MAX = 2 ** (CHAR_BIT - 1) - 1``,
+  `SCHAR_MAX = (UCHAR_MAX - 1) / 2` by SRW_TAC [][type_size_constants] THEN
+  `UCHAR_MAX = 2 ** CHAR_BIT - 1` by SRW_TAC [][type_size_constants] THEN
+  `1n <= 2 ** (CHAR_BIT - 1)` by SRW_TAC [][DECIDE ``1n <= x = 0 < x``] THEN
+  STRIP_ASSUME_TAC CHAR_BIT_BOUNDS THEN
+  SRW_TAC [ARITH_ss][INT_SUB] THEN
+  Q.ABBREV_TAC `C1 = CHAR_BIT - 1` THEN
+  `CHAR_BIT = SUC C1` by SRW_TAC [ARITH_ss][Abbr`C1`] THEN
+  `2n ** CHAR_BIT - 2 = 2 * (2 ** C1 - 1)`
+      by SRW_TAC [][EXP, LEFT_SUB_DISTRIB] THEN
+  METIS_TAC [MULT_DIV, DECIDE ``0n < 2``, MULT_COMM])
+
 val int_representation = prove(
-  ``?rep_int int_value.
+  ``?(rep_int : CPP_Type -> int -> byte list option)
+     (int_value : CPP_Type -> byte list -> int option).
        (!b:byte. int_value (Unsigned Char) [b] = SOME (int_of_num (w2n b))) /\
        (!i. rep_int (Unsigned Char) i =
-              SOME (n2w (Num (i % UCHAR_MAX)))) /\
+              SOME [n2w (Num (i % UCHAR_MAX))]) /\
        (!b. ~word_msb b ==>
             (int_value (Signed Char) [b] = int_value (Unsigned Char) [b])) /\
        (!b. word_msb b ==>
                ?i. (int_value (Signed Char) [b] = SOME i) /\
-                   SCAHR_MIN <= i /\ i <= 0)``,
+                   SCHAR_MIN <= i /\ i <= 0)``,
+  Q.EXISTS_TAC `\ty i. if ty = Unsigned Char then
+                         SOME [n2w (Num (i % UCHAR_MAX))]
+                       else NONE` THEN SIMP_TAC (srw_ss()) [] THEN
+  Q.EXISTS_TAC `\ty bytes. if ty = Unsigned Char then
+                             SOME (&(w2n (HD bytes)))
+                           else if char_onecomp then
+                             if word_msb (HD bytes) then
+                               SOME (~(& (w2n (HD bytes - word_L))))
+                             else SOME (w2i (HD bytes))
+                           else SOME (w2i (HD bytes))` THEN
+  SIMP_TAC (srw_ss()) [] THEN CONJ_TAC THENL [
+    SRW_TAC [][integer_wordTheory.w2i_def],
+    Q.X_GEN_TAC `w` THEN STRIP_TAC THEN
+    Q.ISPEC_THEN `w` STRIP_ASSUME_TAC wordsTheory.ranged_word_nchotomy THEN
+    FULL_SIMP_TAC (srw_ss())
+                  [wordsTheory.word_msb_n2w,
+                   DECIDE ``SUC x - x = 1``,
+                   bitTheory.BIT_def, bitTheory.BITS_def,
+                   bitTheory.MOD_2EXP_def, bitTheory.DIV_2EXP_def] THEN
+    `2 ** (CHAR_BIT - 1) <= n`
+       by (SPOSE_NOT_THEN ASSUME_TAC THEN
+           `n < 2 ** (CHAR_BIT - 1)` by DECIDE_TAC THEN
+           FULL_SIMP_TAC (srw_ss()) [LESS_DIV_EQ_ZERO]) THEN
+    `0 < n` by METIS_TAC [LESS_LESS_EQ_TRANS, bitTheory.ZERO_LT_TWOEXP] THEN
+    `INT_MAX (UNIV : byte_index set) < n`
+       by SRW_TAC [ARITH_ss][integer_wordTheory.INT_MAX_def] THEN
+    `n <= UINT_MAX (UNIV : byte_index set)`
+       by SRW_TAC [ARITH_ss][integer_wordTheory.UINT_MAX_def] THEN
+    SRW_TAC [][integer_wordTheory.w2i_n2w_neg, INT_LE_SUB_RADD,
+               INT_LE_SUB_LADD] THEN
+    `1 <= CHAR_BIT` by (ASSUME_TAC CHAR_BIT THEN DECIDE_TAC) THEN
+    Cases_on `char_onecomp` THEN SRW_TAC [][] THENL [
+      SRW_TAC [][wordsTheory.word_L_def] THEN
+      `SCHAR_MIN = ~SCHAR_MAX`
+        by FULL_SIMP_TAC (srw_ss()) [char_onecomp_def] THEN
+      SRW_TAC [][SCHAR_MAX] THEN
+      SRW_TAC [ARITH_ss][word_sub_n2w_1, bitTheory.MOD_2EXP_LT] THEN
+      SRW_TAC [ARITH_ss][GSYM INT_SUB] THEN
+      Q_TAC SUFF_TAC `2n * (2 ** (CHAR_BIT - 1)) = 2 ** CHAR_BIT` THEN1
+            intLib.ARITH_TAC THEN
+      SRW_TAC [][TWICE_SCHAR_MAX],
+
+      `SCHAR_MIN = ~SCHAR_MAX - 1`
+         by METIS_TAC [char_onecomp_def, type_size_constants] THEN
+      SRW_TAC [][SCHAR_MAX, INT_LE_SUB_LADD] THEN
+      Q.MATCH_ABBREV_TAC `~x + y <= z:int` THEN
+      Q_TAC SUFF_TAC `y <= x + z` THEN1 intLib.ARITH_TAC THEN
+      Q.UNABBREV_ALL_TAC THEN SRW_TAC [][INT_ADD] THEN
+      ASSUME_TAC TWICE_SCHAR_MAX THEN DECIDE_TAC,
+
+      `SCHAR_MIN = ~SCHAR_MAX - 1`
+         by METIS_TAC [char_onecomp_def, type_size_constants] THEN
+      SRW_TAC [][SCHAR_MAX, INT_LE_SUB_RADD]
+    ]
+  ])
+
+val C_INT_REP = new_specification(
+  "C_INT_REP",
+  ["REP_INT", "INT_VAL"],
+  int_representation)
 
 
+(* ----------------------------------------------------------------------
+    calculating type sizes
+
+    This has to be done in conjunction with a map specifying the fields
+    that occur in a struct
+   ---------------------------------------------------------------------- *)
+
+(* -- alignment -- *)
+
+(* alignment of basic integral types *)
+(* ASSUMPTION: basic types will never need to be aligned at boundaries
+               greater than their sizes.
+               For example, if sizeof short == 2, then shorts won't need
+               to be aligned on 4 byte boundaries. *)
+val short_align = new_specification ("short_align",
+  ["short_align"],
+  prove(``?n. 1 <= n /\ n <= short_size``,
+        ASSUME_TAC short_size_nonzero THEN
+        intLib.ARITH_TAC))
+val int_align = new_specification("int_align",
+  ["int_align"],
+  prove(``?n. 1 <= n /\ n <= int_size``,
+        ASSUME_TAC int_size_nonzero THEN
+        intLib.ARITH_TAC))
+val long_align = new_specification("long_align",
+  ["long_align"],
+  prove(``?n. 1 <= n /\ n <= long_size``,
+        ASSUME_TAC long_size_nonzero THEN
+        intLib.ARITH_TAC))
+val ptr_align = new_specification("ptr_align",
+  ["ptr_align"],
+  prove(``?f. !ty. 1 <= f ty /\ f ty <= ptr_size ty /\ (f BChar = f Void)``,
+        Q.EXISTS_TAC `K 1` THEN SRW_TAC [][ptr_size]))
+val bool_align = new_specification("bool_align",
+  ["bool_align"],
+  prove(``?n. 1 <= n /\ n <= bool_size``,
+        ASSUME_TAC bool_size THEN intLib.ARITH_TAC))
+
+(* alignment of the basic integral types *)
+val bit_align = Define`
+  (bit_align Char = 1) /\
+  (bit_align Short = short_align) /\
+  (bit_align Int = int_align) /\
+  (bit_align Long = long_align)
+`;
 
 
+val _ = overload_on ("set", ``list$LIST_TO_SET``)
 
+(* alignment of class types being maximum alignment of member fields is
+   plausible, but should probably count as an ASSUMPTION *)
+val (align_rules, align_ind, align_cases) = Hol_reln`
+  (!smap. align smap BChar 1) /\  (* same as Char *)
 
-val (sizeof_rules, sizeof_induction, sizeof_cases) =
-  IndDefLib.Hol_reln`
+  (!smap. align smap Bool bool_align) /\
 
-(* \#line cholera-model.nw 1088 *)
-(!s b. sizeof s (INL (Signed b)) (bit_size b)) /\
-(!s b. sizeof s (INL (Unsigned b)) (bit_size b)) /\
-(!s t. sizeof s (INL (Ptr t)) ptr_size) /\
-(!s ret args. sizeof s (INL (Function ret args)) fnptr_size)
-(* \#line cholera-model.nw 1046 *)
-                                       /\
+  (!smap ty. align smap (Signed ty) (bit_align ty)) /\
 
-(* \#line cholera-model.nw 1099 *)
-(!s. sizeof s (INR []) 0) /\
-(!s hdt tlt hds tls.
-      sizeof s (INL hdt) hds /\
-      sizeof s (INR tlt) tls ==>
-      sizeof s (INR (hdt :: tlt)) (hds + tls))
-(* \#line cholera-model.nw 1047 *)
-                                       /\
+  (!smap ty. align smap (Unsigned ty) (bit_align ty)) /\
 
-(* \#line cholera-model.nw 1110 *)
-(!s t tsize n. sizeof s (INL t) tsize ==>
-               sizeof s (INL (Array t n)) (tsize * n))
-(* \#line cholera-model.nw 1048 *)
-                                       /\
+  (!smap ty. align smap (Ptr ty) (ptr_align ty)) /\
 
-(* \#line cholera-model.nw 1122 *)
-(!s name sz.
-    sizeof s (INR (MAP SND (s name).struct_info)) sz ==>
-    sizeof s (INL (Struct name)) sz)
-(* \#line cholera-model.nw 1049 *)
-                                        `
-(* \#line cholera-model.nw 1132 *)
-val (sizeof_rewrites0, _) = install_indrel {
-  cases_thm = sizeof_cases,
-  name    = "sizeof",
-  ind_thm = sizeof_induction,
-  position = 2
-};
-val sizeof_rewrites = save_thm(
-  "sizeof_rewrites",
-  LIST_CONJ sizeof_rewrites0);
-(* \#line cholera-model.nw 1051 *)
-local
-  val myth = DB.fetch "choltype"
-  open choltypeTheory
-  val gsz_goal = prove(
-    --`!t. ?n. !s.
-         ((?b. t = Unsigned b) \/ (?b. t = Signed b) \/
-          (?t'. t = Ptr t') \/ (?t' lst. t = Function t' lst)) ==>
-         sizeof s (INL t) n`--,
-    GEN_TAC THEN CONV_TAC EX_OUT_CONV THEN
-    REWRITE_TAC [DISJ_IMP_THM] THEN
-    STRUCT_CASES_TAC (Q.SPEC `t` CType_nchotomy) THEN
-    SIMP_TAC hol_ss [sizeof_rewrites, GSYM CType_distinct, CType_11,
-                     CType_distinct]);
-in
-  val gsizeof = Rsyntax.new_specification {
-    consts = [{const_name = "gsizeof", fixity = Prefix}],
-    name   = "gsizeof",
-    sat_thm = CONV_RULE SKOLEM_CONV gsz_goal}
-end;
-val gsizeof_THM = store_thm(
-  "gsizeof_THM",
-  --`!b t tlst.
-        (gsizeof (Unsigned b) = bit_size b) /\
-        (gsizeof (Signed b) = bit_size b) /\
-        (gsizeof (Ptr t) = ptr_size) /\
-        (gsizeof (Function t tlst) = fnptr_size)`--,
-  REPEAT STRIP_TAC THENL (map (fn t =>
-    ACCEPT_TAC (SIMP_RULE hol_ss [
-      sizeof_rewrites,choltypeTheory.CType_11
-    ] (SPEC t gsizeof))) [--`Unsigned b`--, --`Signed b`--,
-      --`Ptr t`--, --`Function t tlst`--]));
-(* \#line cholera-model.nw 1148 *)
-val sizeof_det_lemma = prove(
-  --`sizeof s t n ==> (\s t n.
-                         !n'. sizeof s t n' ==> (n' = n)) s t n`--,
-  MATCH_MP_TAC sizeof_induction THEN SIMP_TAC hol_ss [] THEN
-  ONCE_REWRITE_TAC [sizeof_rewrites] THEN REPEAT STRIP_TAC THEN
-  RES_TAC THEN ASM_SIMP_TAC hol_ss []);
-val sizeof_det =
-  save_thm("sizeof_det", GEN_ALL (SIMP_RULE hol_ss [] sizeof_det_lemma));
-(* \#line cholera-model.nw 1168 *)
-val declarable_type = new_definition (
-  "declarable_type",
-  ``declarable_type s t = ?n. sizeof s (INL t) n /\ ~(n = 0)``);
-(* \#line cholera-model.nw 1181 *)
-val (offset'_rules, offset'_induction, offset'_cases) = IndDefLib.Hol_reln`
-    (!s n t rest. offset' s (CONS (n,t) rest) n 0n) /\
-    (!s rest n off fsize x xt.
-         sizeof s (INL xt) fsize /\ ~(n = x) /\
-         offset' s rest n off ==>
-         offset' s ((x,xt)::rest) n (fsize + off))`;
-val offset = new_definition (
-  "offset",
-  (--`offset s stid fld off =
-         offset' s (s stid).struct_info fld off`--));
-val (offset'_rewrites, _) = install_indrel {
-  name = "offset'", ind_thm = definition "offset'",
-  position = 2,
-  cases_thm = offset'_cases
-};
-val offset'_rewrites = save_thm(
-  "offset'_rewrites",
-  LIST_CONJ offset'_rewrites);
-val offset'_det = prove(
-  --`!s l fld n. offset' s l fld n ==>
-                 (!n'. offset' s l fld n' ==> (n' = n))`--,
-  HO_MATCH_MP_TAC offset'_induction THEN
-  SIMP_TAC hol_ss [offset'_rewrites] THEN
-  REPEAT STRIP_TAC THEN RES_TAC THEN IMP_RES_TAC sizeof_det THEN
-  ELIM_TAC THEN RWT);
-val offset_det = store_thm (
-  "offset_det",
-  --`!s i fld n. offset s i fld n ==>
-                 !n'. offset s i fld n' ==> (n' = n)`--,
-  SIMP_TAC hol_ss [offset] THEN PROVE_TAC [offset'_det]);
-(* \#line cholera-model.nw 1221 *)
-val wf_type_sizeof = prove(
-  ``!smap vstd t.
-       wf_type smap vstd t ==> ~(t = Void) ==>
-       ?n. sizeof smap (INL t) n``,
-  HO_MATCH_MP_TAC (choltypeTheory.wf_type_strong_induction) THEN
-  SIMP_TAC hol_ss [choltypeTheory.CType_11,
-                    choltypeTheory.CType_distinct] THEN
-  ONCE_REWRITE_TAC [sizeof_rewrites] THEN
-  SIMP_TAC hol_ss [choltypeTheory.str_info_struct_info] THEN
-  REPEAT STRIP_TAC THEN
-  STRIP_ASSUME_TAC
-    (Q.SPEC `smap (sn:string)` (choltypeTheory.str_info_nchotomy)) THEN
-  FULL_SIMP_TAC hol_ss [choltypeTheory.str_info_struct_info] THEN
-  POP_ASSUM_LIST (MAP_EVERY (fn th =>
-    if (free_in ``str_info`` (concl th) orelse
-        free_in ``[]:(string # CType) list`` (concl th)) then
-       ALL_TAC
-    else
-       MP_TAC th)) THEN
-  MAP_EVERY (dub >- SPEC_TAC) [``vstd:string->bool``,
-                               ``l:(string # CType) list``] THEN
-  INDUCT_THEN list_INDUCT STRIP_ASSUME_TAC THEN
-  SIMP_TAC hol_ss [sizeof_rewrites] THEN ASM_MESON_TAC []);
+  (!smap c ty. align smap (MPtr c ty) (ptr_align ty)) (* BAD_ASSUMPTION *) /\
 
-val well_formed_type_sizeof = store_thm(
-  "well_formed_type_sizeof",
-  ``!smap t.
-        well_formed_type smap t ==>
-        ~(t = Void) ==>
-        ?n. sizeof smap (INL t) n``,
-  MESON_TAC [choltypeTheory.well_formed_type, wf_type_sizeof]);
-val sizeof_fn_DEF = Rsyntax.new_specification {
-  consts = [{const_name = "sizeof_fn", fixity = Prefix}],
-  name = "sizeof_fn_DEF",
-  sat_thm = CONV_RULE (rmove_out ``n:num`` THENC SKOLEM_CONV)
-                      well_formed_type_sizeof};
-(* \#line cholera-model.nw 1263 *)
-val ctype_11 = choltypeTheory.CType_11
-val ctype_distinct = let val t = choltypeTheory.CType_distinct
-                     in  CONJ t (GSYM t) end;
-val wf_type_rewrites = choltypeTheory.wf_type_rewrites
-val well_formed_type_THM = choltypeTheory.well_formed_type_THM
-fun start_off (asl, g) =
-  let val lhs_term = lhs g
-      val (_, [smap,cty]) = strip_comb lhs_term
-  in
-      MP_TAC (SPECL [smap, cty] sizeof_fn_DEF) THEN
-      SIMP_TAC hol_ss [ctype_distinct, well_formed_type_THM] THEN
-      ONCE_REWRITE_TAC [sizeof_rewrites, well_formed_type_THM] THEN
-      ASM_SIMP_TAC hol_ss []
-  end (asl, g)
-val ptr_rewrite = prove(
-  ``!smap pt.
-      well_formed_type smap pt ==>
-      (sizeof_fn smap (Ptr pt) = ptr_size)``,
-  REPEAT STRIP_TAC THEN start_off THEN
-  FULL_SIMP_TAC hol_ss [well_formed_type_THM]);
-val num_rewrite = prove(
-  ``(!smap bt. sizeof_fn smap (Signed bt) = bit_size bt) /\
-    (!smap bt. sizeof_fn smap (Unsigned bt) = bit_size bt)``,
-  REPEAT STRIP_TAC THEN start_off);
-val fnptr_rewrite = prove(
-  ``!smap f args.
-       well_formed_type smap f /\ ~array_type f /\
-       EVERY (\t. well_formed_type smap t /\ ~(t = Void) /\
-                  ~array_type t) args ==>
-       (sizeof_fn smap (Function f args) = fnptr_size)``,
-  REPEAT STRIP_TAC THEN start_off THEN
-  FULL_SIMP_TAC hol_ss [well_formed_type_THM, EVERY_MEM]);
-(* \#line cholera-model.nw 1300 *)
-val array_rewrite = prove(
-  ``!smap bt n.
-       well_formed_type smap bt /\ ~(bt = Void) /\ ~(n = 0) ==>
-       (sizeof_fn smap (Array bt n) = n * sizeof_fn smap bt)``,
-  REPEAT STRIP_TAC THEN start_off THEN IMP_RES_TAC sizeof_fn_DEF THEN
-  FULL_SIMP_TAC hol_ss [well_formed_type_THM] THEN STRIP_TAC THEN
-  ASM_SIMP_TAC hol_ss [EQ_MULT_LCANCEL] THEN
-  IMP_RES_TAC sizeof_det);
-(* \#line cholera-model.nw 1315 *)
-val struct_rewrite = prove(
-  ``!smap sn.
-       well_formed_type smap (Struct sn) ==>
-       (sizeof_fn smap (Struct sn) =
-          FOLDR (\x y. sizeof_fn smap x + y)
-                0
-                (MAP SND (smap sn).struct_info))``,
-  REPEAT GEN_TAC THEN DISCH_THEN (fn th =>
-    MP_TAC th THEN
-    MP_TAC (MATCH_MP (REWRITE_RULE [GSYM IMP2_THM] sizeof_fn_DEF) th))
-  THEN SIMP_TAC hol_ss [ctype_distinct] THEN
-  ONCE_REWRITE_TAC [sizeof_rewrites] THEN REPEAT STRIP_TAC THEN
-  FULL_SIMP_TAC hol_ss [choltypeTheory.str_info_struct_info,
-                         well_formed_type_THM,
-                         pred_setTheory.NOT_IN_EMPTY] THEN
-  POP_ASSUM_LIST (MAP_EVERY (fn th =>
-    if (free_in ``nodup_flds`` (concl th) orelse
-        free_in ``[]:(string # CType) list`` (concl th) orelse
-        free_in ``wf_type`` (concl th)) then
-       ALL_TAC
-    else MP_TAC th)) THEN
-  SPEC_TAC (``sizeof_fn smap (Struct sn)``, ``n:num``) THEN
-  REPEAT_TCL STRIP_THM_THEN SUBST_ALL_TAC
-    (Q.SPEC `smap (sn:string)`
-           (choltypeTheory.str_info_nchotomy)) THEN
-  SIMP_TAC hol_ss [choltypeTheory.str_info_struct_info] THEN
-  SPEC_TAC (dub ``l:(string # CType) list``) THEN
-  INDUCT_THEN list_INDUCT ASSUME_TAC THENL [
-    SIMP_TAC hol_ss [sizeof_rewrites],
-    SIMP_TAC hol_ss [sizeof_rewrites, well_formed_type_THM,
-                      DISJ_IMP_THM, FORALL_AND_THM] THEN
-    REPEAT STRIP_TAC THEN IMP_RES_TAC sizeof_fn_DEF THEN
-    POP_ASSUM (GSYM >- ASSUME_TAC) THEN
-    FIRST_X_ASSUM (res_search false [] []) THEN
-    res_search_then true [] [] SUBST_ALL_TAC sizeof_det THEN
-    ELIM_TAC THEN FULL_SIMP_TAC hol_ss [sizeof_rewrites]
-  ]);
-(* \#line cholera-model.nw 1358 *)
-val sizeof_fn = save_thm(
-  "sizeof_fn",
-  LIST_CONJ [num_rewrite, ptr_rewrite, fnptr_rewrite, struct_rewrite,
-             array_rewrite]);
-(* \#line cholera-model.nw 1368 *)
-val wf_type_offset = store_thm(
-  "wf_type_offset",
-  ``!smap sn. well_formed_type smap (Struct sn) ==>
-              !fld t. lookup_field_info (smap sn) fld t ==>
-                      ?n. offset smap sn fld n``,
-  SIMP_TAC (hol_ss ++ impnorm_set) [offset,
-    choltypeTheory.lookup_field_info,
-    choltypeTheory.str_info_struct_info] THEN
-  REPEAT STRIP_TAC THEN
-  IMP_RES_TAC (choltypeTheory.well_formed_structs) THEN
-  FULL_SIMP_TAC hol_ss [well_formed_type_THM] THEN
-  FIRST_X_ASSUM SUBST_ALL_TAC THEN
-  FULL_SIMP_TAC hol_ss [choltypeTheory.str_info_struct_info] THEN
-  POP_ASSUM_LIST (MAP_EVERY (fn th =>
-    if (free_in ``nodup_flds`` (concl th) orelse
-        free_in ``[]:(string # CType) list`` (concl th)) then
-       ALL_TAC
-    else MP_TAC th)) THEN
-  SPEC_TAC (dub ``l:(string # CType) list``) THEN
-  INDUCT_THEN list_INDUCT ASSUME_TAC THEN SIMP_TAC hol_ss [] THEN
-  GEN_TAC THEN
-  STRUCT_CASES_TAC (ISPEC ``h:string # CType`` pair_CASES) THEN
-  SIMP_TAC hol_ss [DISJ_IMP_THM, GSYM RIGHT_FORALL_IMP_THM,
-                   FORALL_AND_THM] THEN
-  ONCE_REWRITE_TAC [offset'_rewrites] THEN REPEAT STRIP_TAC THEN
-  ASM_MESON_TAC [well_formed_type_sizeof]);
-(* \#line cholera-model.nw 1402 *)
-val bit_cases = choltypeTheory.basic_integral_type_nchotomy
-val bit_size_nonzero = store_thm(
-  "bit_size_nonzero",
-  --`!b. ~(bit_size b = 0)`--,
-  GEN_TAC THEN STRUCT_CASES_TAC (Q.SPEC `b` bit_cases) THEN
-  SIMP_TAC hol_ss [bit_size] THEN
-  STRIP_ASSUME_TAC (choltypeTheory.type_size_constants) THENL
-  (map (fn th =>
-    ASSUME_TAC th THEN STRIP_TAC THEN POP_ASSUM SUBST_ALL_TAC THEN
-    FULL_SIMP_TAC hol_ss [integerTheory.INT_EXP_CALCULATE] THEN
-    POP_ASSUM (fn th =>
-       Q.PAT_ASSUM `^(rand (rator (concl th))) = X`
-         (fn th2 => ASSUME_TAC th THEN SUBST_ALL_TAC th2)) THEN
-    IMP_RES_THEN IMP_RES_TAC integerTheory.INT_LE_TRANS THEN
-    FULL_SIMP_TAC (hol_ss ++ intSimps.INT_REDUCE_ss) [])
-   [short_size, int_size, long_size]));
-(* \#line cholera-model.nw 1421 *)
-val simple_arith = ARITH_PROVE (--`!c:num. 1 <= c ==> ~(c = 0)`--)
-val sizeof_not_zero_lemma = prove(
-  ``!smap x n.
-       sizeof smap x n ==>
-       (!t. (x = INL t) ==> well_formed_type smap t ==>
-            ~(t = Void) ==> ~(n = 0)) /\
-       (!tl. (x = INR tl) ==> ~(tl = []) ==>
-             EVERY (well_formed_type smap) tl ==>
-             EVERY ($~ o $= Void) tl ==> ~(n = 0))``,
-  HO_MATCH_MP_TAC sizeof_induction THEN
-  REPEAT CONJ_TAC THEN SIMP_TAC hol_ss [ctype_distinct,
-    sizeof_rewrites, bit_size_nonzero, ptr_size, simple_arith,
-    fnptr_size, combinTheory.o_THM]
-  THENL [
-    SIMP_TAC hol_ss [well_formed_type_THM] THEN
-    REPEAT GEN_TAC THEN STRIP_TAC THEN GEN_TAC THEN
-    REPEAT_TCL STRIP_THM_THEN SUBST_ALL_TAC
-      (Q.SPEC `n` num_CASES) THEN
-    FULL_SIMP_TAC hol_ss [RIGHT_ADD_DISTRIB, LEFT_ADD_DISTRIB,
-                           MULT_CLAUSES] THEN
-    STRIP_TAC THEN RES_TAC THEN FULL_SIMP_TAC hol_ss [],
-    SIMP_TAC hol_ss [EVERY_MEM, EXISTS_MEM, combinTheory.o_THM] THEN
-    REPEAT STRIP_TAC THEN IMP_RES_TAC (choltypeTheory.well_formed_structs) THEN
-    FULL_SIMP_TAC hol_ss [well_formed_type_THM]
-  ]);
-val sizeof_not_zero = save_thm(
-  "sizeof_not_zero",
-  CONJUNCT1 (SIMP_RULE (hol_ss ++ impnorm_set) [
-      GSYM RIGHT_FORALL_IMP_THM, FORALL_AND_THM]
-  sizeof_not_zero_lemma));
-val sizeof_fn_not_zero = store_thm(
-  "sizeof_fn_not_zero",
-  ``!smap t. well_formed_type smap t /\ ~(t = Void) ==>
-             ~(sizeof_fn smap t = 0)``,
-  REPEAT STRIP_TAC THEN IMP_RES_TAC sizeof_fn_DEF THEN
-  FIRST_X_ASSUM SUBST_ALL_TAC THEN ASM_MESON_TAC [sizeof_not_zero]);
-(* \#line cholera-model.nw 1481 *)
-val convert_unsigned = new_definition (
-  "convert_unsigned",
-  --`convert_unsigned (v:MemObj list) t1 t2 =
-       let len1 = gsizeof t1 in
-       let len2 = gsizeof t2 in
-         (len1 > len2 => LASTN len2 v
-                      |  APPEND (num2mval (len2 - len1) 0) v)`--);
-val convert_unsigned_same_types = store_thm(
-  "convert_unsigned_same_types",
-  ``!v t1. convert_unsigned v t1 t1 = v``,
-  SIMP_TAC hol_ss [LET_THM, convert_unsigned, num2mval, split2bytes]);
-val bit_less_than = new_definition (
-  "bit_less_than",
-  ``bit_less_than bt1 bt2 =
-      (bt1 = Char) /\ ~(bt2 = Char) \/
-      (bt1 = Short) /\ ~(bt2 IN {Char; Short}) \/
-      (bt1 = Int) /\ (bt2 = Long)``);
-val convert_signed2unsigned = new_definition(
-  "convert_signed2unsigned",
-  ``convert_signed2unsigned (v1, bt1) (v2, bt2) =
-      ?n. n < 2 EXP (CHAR_BIT * bit_size bt1) /\
-          (v1 = num2mval (bit_size bt1) n) /\
-          (v2 = num2mval (bit_size bt2) n)``);
-val convert_val = new_definition (
-  "convert_val",
-  --`convert_val s (v1, t1) (v2, t2) =
-       (sizeof s (INL t1) (LENGTH v1) \/ (t1 = Void) /\ (v1 = [])) /\
-       ((?bt. t1 = Unsigned bt) /\ (?bt. t2 = Unsigned bt) /\
-        (v2 = convert_unsigned v1 t1 t2) \/
-        (?bt1 bt2. (t1 = Signed bt1) /\ (t2 = Unsigned bt2) /\
-                   convert_signed2unsigned (v1, bt1) (v2, bt2)) \/
-        pointer_type t1 /\ pointer_type t2 /\ (v2 = v1) \/
-        (t1 = t2) /\ (v2 = v1) \/
-        (t2 = Void) /\ (v2 = []))`--);
-(* \#line cholera-model.nw 1526 *)
-val RES_FORALL = res_quanTheory.RES_FORALL
-val len_split2bytes = store_thm(
-  "len_split2bytes",
-  --`!n w:'a word. LENGTH (split2bytes n w) = n`--,
-  numLib.INDUCT_TAC THEN
-  ASM_SIMP_TAC hol_ss [split2bytes, rich_listTheory.LENGTH_SNOC]);
-val len_num2mval = store_thm(
-  "len_num2mval",
-  --`!l n. LENGTH (num2mval l n) = l`--,
-  numLib.INDUCT_TAC THEN ASM_SIMP_TAC hol_ss [num2mval, len_split2bytes]);
-val FOLDL_MAP = prove(
-  (--`!(f:'a->'b->'a) (g:'c->'b) l e.
-         FOLDL f e (MAP g l) = FOLDL (\x y. f x (g y)) e l`--),
-  REPEATN 2 GEN_TAC THEN SingleStep.Induct THEN
-  ASM_SIMP_TAC hol_ss []);
-val BNVAL_WCAT =
-  CONV_RULE (SIMP_CONV hol_ss [word_baseTheory.PWORDLEN, RES_FORALL])
-            bword_numTheory.BNVAL_WCAT
-open SingleStep
-infix 8 by
-infix |->
-val LESS_DIV = prove(
-  (--`!x y z. 0 < y /\ x < y * z ==> x DIV y < z`--),
-  REPEAT STRIP_TAC THEN
-  `~(y = 0)` by ASM_SIMP_TAC hol_ss [] THEN
-  POP_ASSUM (fn th =>
-    `?n. y = SUC n` by ASM_MESON_TAC [arithmeticTheory.num_CASES, th]) THEN
-  POP_ASSUM SUBST_ALL_TAC THEN
-  CONV_TAC (K (SYM (INST
-                      [(--`m:num`--) |-> (--`x DIV (SUC n)`--),
-                       (--`i:num`--) |-> (--`z:num`--)]
-                    (SPEC_ALL arithmeticTheory.LESS_MULT_MONO)))) THEN
-  CONV_TAC (arg_CONV 1 (REWR_CONV arithmeticTheory.MULT_SYM)) THEN
-  ASSUME_TAC (CONJUNCT1 (SPEC (--`x:num`--)
-                        (MATCH_MP DIVISION
-                                  (ASSUME (--`0 < SUC n`--))))) THEN
-  IMP_RES_TAC (ARITH_PROVE (--`(x:num = y + z) ==> (y <= x)`--)) THEN
-  POP_ASSUM (STRIP_ASSUME_TAC o
-             REWRITE_RULE [arithmeticTheory.LESS_OR_EQ]) THENL [
-    ASM_MESON_TAC [arithmeticTheory.LESS_TRANS],
-    ASM_SIMP_TAC hol_ss []
-  ]);
-val WSPLIT_WCAT = prove(
-  (--`!x y n. (WORDLEN (x:'a word) = n) ==>
-              (WSPLIT n (WCAT(y,x)) = (y,x))`--),
+  (!smap ty n a. align smap ty a ==> align smap (Array ty n) a) /\
+
+  (!smap cnm max.
+      cnm IN FDOM smap /\
+      (!ty. ty IN set (smap ' cnm) ==>
+            ?a. align smap ty a /\ a <= max) /\
+      (?ty. ty IN set (smap ' cnm) /\ align smap ty max)
+         ==>
+      align smap (Class cnm) max)
+
+`;
+
+(* SANITY : alignment relation is deterministic *)
+val align_det = store_thm(
+  "align_det",
+  ``!smap ty a. align smap ty a ==>
+                !b. align smap ty b ==> (a = b)``,
+  HO_MATCH_MP_TAC align_ind THEN REPEAT CONJ_TAC THEN
   REPEAT GEN_TAC THEN
-  MAP_EVERY (fn t => REPEAT_TCL STRIP_THM_THEN SUBST1_TAC
-                     (ISPEC t word_baseTheory.word_cases))
-            [(--`x:'a word`--), (--`y:'a word`--)] THEN
-  let open wordTheory word_baseTheory
-  in
-    REWRITE_TAC [WORDLEN_DEF, WCAT_DEF, WSPLIT_DEF, PAIR_EQ, WORD_11]
-  end THEN REPEAT STRIP_TAC THEN
-  IMP_RES_TAC (ARITH_PROVE (--`(x = n:num) ==> (x <= n)`--)) THENL [
-    ASM_SIMP_TAC hol_ss [rich_listTheory.BUTLASTN_APPEND1,
-                         rich_listTheory.BUTLASTN],
-    ASM_SIMP_TAC hol_ss [rich_listTheory.LASTN_APPEND1,
-                         rich_listTheory.LASTN]
-  ]);
-val mult_over_add = prove(
-  (--`(!x:num y z. x * (y + z) = x * y + x * z) /\
-      (!x:num y z. (y + z) * x = x * y + x * z)`--),
-  CONV_TAC (conj2_CONV (STRIP_QUANT_CONV (lhs_CONV
-    (REWR_CONV (arithmeticTheory.MULT_SYM))))) THEN RWT THEN
-  numLib.INDUCT_TAC THENL [
-    REWRITE_TAC [arithmeticTheory.ADD_CLAUSES, arithmeticTheory.MULT_CLAUSES],
-    ONCE_REWRITE_TAC [arithmeticTheory.MULT_SYM] THEN
-    REWRITE_TAC [arithmeticTheory.MULT_SUC] THEN
-    ONCE_REWRITE_TAC [arithmeticTheory.MULT_SYM] THEN ARWT THEN
-    REPEAT GEN_TAC THEN CONV_TAC ARITH_CONV
-  ]);
-val two_exp_gt_zero = prove(
-  ``!n. 0 < 2 EXP n``,
-  SIMP_TAC hol_ss [ARITH_PROVE ``0n < n = ~(n = 0)``] THEN
-  REWRITE_TAC [ARITH_PROVE ``2 = SUC 1``, NOT_EXP_0])
-local
-  open bword_numTheory
-  val BNVAL_WCAT =
-    CONV_RULE (SIMP_CONV hol_ss [word_baseTheory.PWORDLEN, RES_FORALL])
-               bword_numTheory.BNVAL_WCAT
-in
-  val num2mval_safe = store_thm(
-    "num2mval_safe",
-    ``!nb n. (n < 2 EXP (CHAR_BIT * nb)) ==>
-               (coerce_to_num (num2mval nb n) = n)``,
-    SIMP_TAC hol_ss [coerce_to_num, num2mval, obj2byte, FOLDL_MAP,
-                     pairTheory.CURRY_DEF] THEN Induct
-    THENL [
-      SIMP_TAC hol_ss [MULT_CLAUSES] THEN REPEAT STRIP_TAC THEN
-      IMP_RES_TAC (ARITH_PROVE (--`n < 1n ==> (n = 0)`--)) THEN
-      ELIM_TAC THEN SIMP_TAC hol_ss [split2bytes,
-                                     bword_numTheory.BNVAL0],
-      SIMP_TAC bool_ss [MULT_CLAUSES, NBWORD_SPLIT, WSPLIT_WCAT,
-                        WORDLEN_NBWORD, split2bytes] THEN
-      SIMP_TAC hol_ss [rich_listTheory.FOLDL_SNOC, BNVAL_WCAT] THEN
-      ONCE_REWRITE_TAC [
-        GSYM (SPEC ``CHAR_BIT`` bword_numTheory.NBWORD_MOD)] THEN
-      SIMP_TAC hol_ss [bword_numTheory.BNVAL_NBWORD, DIVISION, two_exp_gt_zero,
-                       arithmeticTheory.EXP_ADD] THEN
-      REPEAT STRIP_TAC THEN
-      ASM_SIMP_TAC hol_ss [LESS_DIV, two_exp_gt_zero, WORDLEN_NBWORD] THEN
-      SYM_TAC THEN
-      ACCEPT_TAC (CONJUNCT1
-        (SPEC ``n:num``
-              (MATCH_MP DIVISION (SPEC ``CHAR_BIT`` two_exp_gt_zero))))
-    ])
-end;
-(* \#line cholera-model.nw 1639 *)
-val convert_val_det = store_thm(
-  "convert_val_det",
-  ``!s v1 t1 v2 t2.
-          convert_val s (v1, t1) (v2, t2) ==>
-          !v'. convert_val s (v1, t1) (v', t2) ==> (v' = v2)``,
-  SIMP_TAC hol_ss [convert_val] THEN REPEAT STRIP_TAC THEN
-  ELIM_TAC THEN FULL_SIMP_TAC hol_ss [
-    choltypeTheory.pointer_type, convert_unsigned_same_types,
-    convert_signed2unsigned, pred_setTheory.IN_INSERT,
-    pred_setTheory.NOT_IN_EMPTY, choltypeTheory.CType_11,
-    choltypeTheory.CType_distinct] THEN
-  RULE_ASSUM_TAC (ONCE_REWRITE_RULE [sizeof_cases]) THEN
-  FULL_SIMP_TAC hol_ss [choltypeTheory.CType_distinct,
-                         choltypeTheory.CType_11] THEN
-  ELIM_TAC THEN ARWT THEN
-  FIRST_X_ASSUM (AP_TERM ``coerce_to_num`` >- MP_TAC) THEN
-  ASM_SIMP_TAC hol_ss [num2mval_safe]);
-val convert_preserves_sizes = store_thm(
-  "convert_preserves_sizes",
-  --`!vt v2 t2 s. convert_val s vt (v2, t2) ==> ~(t2 = Void) ==>
-                  sizeof s (INL t2) (LENGTH v2)`--,
-  REPEAT GEN_TAC THEN CONV_TAC (ant_CONV (arg_CONV 2 pair_CONV)) THEN
-  SIMP_TAC hol_ss [convert_val] THEN REPEAT STRIP_TAC THEN
-  ELIM_TAC THEN FULL_SIMP_TAC hol_ss [] THENL [
-    FULL_SIMP_TAC hol_ss [
-      sizeof_rewrites, convert_unsigned, gsizeof_THM, LET_THM] THEN
-    COND_CASES_TAC THEN ASM_SIMP_TAC hol_ss [
-      rich_listTheory.LENGTH_LASTN, LENGTH_APPEND, len_num2mval],
-    FULL_SIMP_TAC hol_ss [convert_signed2unsigned, len_num2mval,
-                           sizeof_rewrites],
-    FULL_SIMP_TAC hol_ss [choltypeTheory.pointer_type,
-      sizeof_rewrites] THEN ELIM_TAC THEN
-    FIRST_ASSUM SUBST_ALL_TAC THEN
-    FULL_SIMP_TAC hol_ss [sizeof_rewrites],
-    FULL_SIMP_TAC hol_ss [choltypeTheory.CType_distinct],
-    FULL_SIMP_TAC hol_ss [convert_signed2unsigned, len_num2mval,
-                           sizeof_rewrites],
-    REPEAT (FIRST_X_ASSUM SUBST_ALL_TAC) THEN
-    FULL_SIMP_TAC hol_ss [choltypeTheory.CType_distinct,
-      choltypeTheory.pointer_type]
-  ]);
-(* \#line cholera-model.nw 713 *)
+  ((Q.MATCH_ABBREV_TAC `align X Y Z ==> P` THEN
+    Q.UNABBREV_ALL_TAC THEN
+    ONCE_REWRITE_TAC [align_cases]) ORELSE
+   (STRIP_TAC THEN ONCE_REWRITE_TAC [align_cases])) THEN
+  SRW_TAC [][] THEN
+  FULL_SIMP_TAC (srw_ss()) [listTheory.IN_LIST_TO_SET] THEN
+  METIS_TAC [DECIDE ``a:num <= b /\ b <= a ==> (a = b)``])
+
+
+(* ----------------------------------------------------------------------
+    type sizes and field offsets within classes
+   ---------------------------------------------------------------------- *)
+
+val roundup_def = Define`
+  roundup base n = if n MOD base = 0 then n else (n DIV base + 1) * base
+`;
+
+val (offsizeof_rules, offsizeof_ind, offsizeof_cases) = Hol_reln`
+
+  (!s. sizeof s BChar 1) /\
+
+  (!s. sizeof s Bool bool_size) /\
+
+  (!s b. sizeof s (Signed b) (bit_size b)) /\
+
+  (!s b. sizeof s (Unsigned b) (bit_size b)) /\
+
+  (!s t. sizeof s (Ptr t) (ptr_size t)) /\
+
+  (!s c t. sizeof s (MPtr c t) (ptr_size t)) /\ (* BAD_ASSUMPTION *)
+
+  (!s m n t. sizeof s t m ==> sizeof s (Array t n) (m * n)) /\
+
+  (!s c tylist a lastoff lastsz.
+        c IN FDOM s /\ (s ' c = tylist) /\
+        align s (Class c) a /\
+        offset s tylist (LENGTH tylist - 1) lastoff /\
+        sizeof s (EL (LENGTH tylist - 1) tylist) lastsz
+      ==>
+        sizeof s (Class c) (roundup a (lastoff + lastsz))) /\
+
+  (!s tylist.  offset s tylist 0 0) /\
+  (!s tylist n a offn sizen.
+        offset s tylist n offn /\
+        sizeof s (EL n tylist) sizen /\
+        align s (EL (SUC n) tylist) a
+      ==>
+        offset s tylist (SUC n) (roundup a (offn + sizen)))
+`;
+
+
+(* SANITY: sizeof and offset are deterministic *)
+val det_lemma = prove(
+  ``(!s ty n. sizeof s ty n ==> !m. sizeof s ty m ==> (n = m)) /\
+    (!s tylist n off1.
+              offset s tylist n off1 ==>
+              !off2. offset s tylist n off2 ==> (off1 = off2))``,
+  HO_MATCH_MP_TAC offsizeof_ind THEN REPEAT CONJ_TAC THEN
+  REPEAT GEN_TAC THENL [
+    ONCE_REWRITE_TAC [offsizeof_cases] THEN SRW_TAC [][],
+    ONCE_REWRITE_TAC [offsizeof_cases] THEN SRW_TAC [][],
+    ONCE_REWRITE_TAC [offsizeof_cases] THEN SRW_TAC [][],
+    ONCE_REWRITE_TAC [offsizeof_cases] THEN SRW_TAC [][],
+    ONCE_REWRITE_TAC [offsizeof_cases] THEN SRW_TAC [][],
+    ONCE_REWRITE_TAC [offsizeof_cases] THEN SRW_TAC [][],
+    (* array *)
+    STRIP_TAC THEN ONCE_REWRITE_TAC [offsizeof_cases] THEN SRW_TAC [][] THEN
+    METIS_TAC [],
+    (* class size *)
+    STRIP_TAC THEN ONCE_REWRITE_TAC [offsizeof_cases] THEN SRW_TAC [][] THEN
+    METIS_TAC [align_det],
+    (* offset 0 *)
+    ONCE_REWRITE_TAC [offsizeof_cases] THEN SRW_TAC [][],
+    (* offset SUC *)
+    STRIP_TAC THEN ONCE_REWRITE_TAC [offsizeof_cases] THEN SRW_TAC [][] THEN
+    METIS_TAC [align_det, listTheory.EL]
+  ])
+val sizeof_det = save_thm("sizeof_det", CONJUNCT1 det_lemma)
+val offset_det = save_thm("offset_det", CONJUNCT2 det_lemma)
+
 val _ = export_theory();
